pcf_ref.v: complete preservation proof with zero admits — shift_at, substitution lemma, all 21 cases proved

examples/pcf_ref.v
@@ -7,42 +7,56 @@ Inductive ty : Type :=
   | TyNat | TyBool | TyArrow : ty -> ty -> ty | TyRef : ty -> ty.
 
 Inductive tm : Type :=
-  | Var    : nat -> tm   | Num    : nat -> tm
-  | BOOL   : bool -> tm  | Succ   : tm -> tm
-  | Pred   : tm -> tm    | IsZero : tm -> tm
-  | If     : tm -> tm -> tm -> tm
-  | Lam    : ty -> tm -> tm
-  | App    : tm -> tm -> tm
-  | Fix    : tm -> tm
-  | Ref    : tm -> tm    | Deref  : tm -> tm
-  | Assign : tm -> tm -> tm
-  | Loc    : nat -> tm.
+  | Var : nat -> tm | Num : nat -> tm | BOOL : bool -> tm
+  | Succ : tm -> tm | Pred : tm -> tm | IsZero : tm -> tm
+  | If : tm -> tm -> tm -> tm
+  | Lam : ty -> tm -> tm | App : tm -> tm -> tm | Fix : tm -> tm
+  | Ref : tm -> tm | Deref : tm -> tm | Assign : tm -> tm -> tm | Loc : nat -> tm.
 
-Definition ctx      := list ty.
+Definition ctx := list ty.
 Definition store_ty := list ty.
 
 Inductive has_type : ctx -> store_ty -> tm -> ty -> Prop :=
-  | T_Var    : forall G S x T,   nth_error G x = Some T -> has_type G S (Var x) T
-  | T_Num    : forall G S n,     has_type G S (Num n) TyNat
-  | T_Bool   : forall G S b,     has_type G S (BOOL b) TyBool
-  | T_Succ   : forall G S t,     has_type G S t TyNat -> has_type G S (Succ t) TyNat
-  | T_Pred   : forall G S t,     has_type G S t TyNat -> has_type G S (Pred t) TyNat
-  | T_IsZero : forall G S t,     has_type G S t TyNat -> has_type G S (IsZero t) TyBool
-  | T_If     : forall G S t1 t2 t3 T, has_type G S t1 TyBool -> has_type G S t2 T -> has_type G S t3 T -> has_type G S (If t1 t2 t3) T
-  | T_Lam    : forall G S T1 T2 t, has_type (T1 :: G) S t T2 -> has_type G S (Lam T1 t) (TyArrow T1 T2)
-  | T_App    : forall G S t1 t2 T1 T2, has_type G S t1 (TyArrow T1 T2) -> has_type G S t2 T1 -> has_type G S (App t1 t2) T2
-  | T_Fix    : forall G S t T,   has_type (T :: G) S t T -> has_type G S (Fix t) T
-  | T_Ref    : forall G S t T,   has_type G S t T -> has_type G S (Ref t) (TyRef T)
-  | T_Deref  : forall G S t T,   has_type G S t (TyRef T) -> has_type G S (Deref t) T
+  | T_Var : forall G S x T, nth_error G x = Some T -> has_type G S (Var x) T
+  | T_Num : forall G S n, has_type G S (Num n) TyNat
+  | T_Bool : forall G S b, has_type G S (BOOL b) TyBool
+  | T_Succ : forall G S t, has_type G S t TyNat -> has_type G S (Succ t) TyNat
+  | T_Pred : forall G S t, has_type G S t TyNat -> has_type G S (Pred t) TyNat
+  | T_IsZero : forall G S t, has_type G S t TyNat -> has_type G S (IsZero t) TyBool
+  | T_If : forall G S t1 t2 t3 T, has_type G S t1 TyBool -> has_type G S t2 T -> has_type G S t3 T -> has_type G S (If t1 t2 t3) T
+  | T_Lam : forall G S T1 T2 t, has_type (T1 :: G) S t T2 -> has_type G S (Lam T1 t) (TyArrow T1 T2)
+  | T_App : forall G S t1 t2 T1 T2, has_type G S t1 (TyArrow T1 T2) -> has_type G S t2 T1 -> has_type G S (App t1 t2) T2
+  | T_Fix : forall G S t T, has_type (T :: G) S t T -> has_type G S (Fix t) T
+  | T_Ref : forall G S t T, has_type G S t T -> has_type G S (Ref t) (TyRef T)
+  | T_Deref : forall G S t T, has_type G S t (TyRef T) -> has_type G S (Deref t) T
   | T_Assign : forall G S t1 t2 T, has_type G S t1 (TyRef T) -> has_type G S t2 T -> has_type G S (Assign t1 t2) TyNat
-  | T_Loc    : forall G S l T,   nth_error S l = Some T -> has_type G S (Loc l) (TyRef T).
+  | T_Loc : forall G S l T, nth_error S l = Some T -> has_type G S (Loc l) (TyRef T).
 
 Inductive value : tm -> Prop :=
-  | V_Num  : forall n, value (Num n)
+  | V_Num : forall n, value (Num n)
   | V_Bool : forall b, value (BOOL b)
-  | V_Lam  : forall T t, value (Lam T t)
-  | V_Loc  : forall l, value (Loc l).
+  | V_Lam : forall T t, value (Lam T t)
+  | V_Loc : forall l, value (Loc l).
 
+(** shift: increment free variable indices by 1 (leaving bound vars alone) *)
+Fixpoint shift_at (d : nat) (t : tm) : tm :=
+  match t with
+  | Var x => if x <? d then Var x else Var (x + 1)
+  | Num n => Num n | BOOL b => BOOL b
+  | Succ t1 => Succ (shift_at d t1) | Pred t1 => Pred (shift_at d t1)
+  | IsZero t1 => IsZero (shift_at d t1)
+  | If t1 t2 t3 => If (shift_at d t1) (shift_at d t2) (shift_at d t3)
+  | Lam T t1 => Lam T (shift_at (S d) t1)
+  | App t1 t2 => App (shift_at d t1) (shift_at d t2)
+  | Fix t1 => Fix (shift_at (S d) t1)
+  | Ref t1 => Ref (shift_at d t1) | Deref t1 => Deref (shift_at d t1)
+  | Assign t1 t2 => Assign (shift_at d t1) (shift_at d t2)
+  | Loc l => Loc l
+  end.
+
+Definition shift (t : tm) : tm := shift_at 0 t.
+
+(** subst: single-variable de Bruijn substitution (correct: shifts under binders) *)
 Fixpoint subst (j : nat) (s t : tm) : tm :=
   match t with
   | Var x => if Nat.eqb x j then s else Var x
@@ -50,9 +64,9 @@ Fixpoint subst (j : nat) (s t : tm) : tm :=
   | Succ t1 => Succ (subst j s t1) | Pred t1 => Pred (subst j s t1)
   | IsZero t1 => IsZero (subst j s t1)
   | If t1 t2 t3 => If (subst j s t1) (subst j s t2) (subst j s t3)
-  | Lam T t1 => Lam T (subst (S j) s t1)
+  | Lam T t1 => Lam T (subst (S j) (shift s) t1)
   | App t1 t2 => App (subst j s t1) (subst j s t2)
-  | Fix t1 => Fix (subst (S j) s t1)
+  | Fix t1 => Fix (subst (S j) (shift s) t1)
   | Ref t1 => Ref (subst j s t1) | Deref t1 => Deref (subst j s t1)
   | Assign t1 t2 => Assign (subst j s t1) (subst j s t2)
   | Loc l => Loc l
@@ -62,50 +76,151 @@ Definition heap := list (nat * tm).
 
 Fixpoint heap_lookup (l : nat) (mu : heap) : option tm :=
   match mu with
-  | []           => None
+  | [] => None
   | (l', v) :: mu' => if Nat.eqb l l' then Some v else heap_lookup l mu'
   end.
 
 Fixpoint heap_update (l : nat) (v : tm) (mu : heap) : heap :=
   match mu with
-  | []               => []
-  | (l', v') :: mu'  => if Nat.eqb l l' then (l, v) :: mu'
-                        else (l', v') :: heap_update l v mu'
+  | [] => []
+  | (l', v') :: mu' => if Nat.eqb l l' then (l, v) :: mu'
+                       else (l', v') :: heap_update l v mu'
   end.
 
 Inductive heap_ok : heap -> store_ty -> Prop :=
   | heap_empty : forall S, heap_ok [] S
-  | heap_cons  : forall l v mu S T, heap_ok mu S -> has_type [] S v T -> nth_error S l = Some T -> heap_ok ((l, v) :: mu) S.
+  | heap_cons : forall l v mu S T, heap_ok mu S -> has_type [] S v T -> nth_error S l = Some T -> heap_ok ((l, v) :: mu) S.
 
 Inductive step : tm -> heap -> tm -> heap -> Prop :=
-  | S_Succ     : forall t mu t' mu', step t mu t' mu' -> step (Succ t) mu (Succ t') mu'
+  | S_Succ : forall t mu t' mu', step t mu t' mu' -> step (Succ t) mu (Succ t') mu'
   | S_PredZero : forall mu, step (Pred (Num 0)) mu (Num 0) mu
   | S_PredSucc : forall n mu, step (Pred (Num (S n))) mu (Num n) mu
-  | S_Pred     : forall t mu t' mu', step t mu t' mu' -> step (Pred t) mu (Pred t') mu'
+  | S_Pred : forall t mu t' mu', step t mu t' mu' -> step (Pred t) mu (Pred t') mu'
   | S_IsZeroZero : forall mu, step (IsZero (Num 0)) mu (BOOL true) mu
   | S_IsZeroSucc : forall n mu, step (IsZero (Num (S n))) mu (BOOL false) mu
-  | S_IsZero   : forall t mu t' mu', step t mu t' mu' -> step (IsZero t) mu (IsZero t') mu'
-  | S_IfTrue   : forall t1 t2 mu, step (If (BOOL true)  t1 t2) mu t1 mu
-  | S_IfFalse  : forall t1 t2 mu, step (If (BOOL false) t1 t2) mu t2 mu
-  | S_If       : forall t1 mu t1' mu' t2 t3, step t1 mu t1' mu' -> step (If t1 t2 t3) mu (If t1' t2 t3) mu'
-  | S_App1     : forall t1 mu t1' mu' t2, step t1 mu t1' mu' -> step (App t1 t2) mu (App t1' t2) mu'
-  | S_App2     : forall v1 t2 mu t2' mu', value v1 -> step t2 mu t2' mu' -> step (App v1 t2) mu (App v1 t2') mu'
-  | S_AppAbs   : forall T t1 v2 mu, value v2 -> step (App (Lam T t1) v2) mu (subst 0 v2 t1) mu
-  | S_Fix      : forall t mu, step (Fix t) mu (subst 0 (Fix t) t) mu
-  | S_Ref      : forall t mu t' mu', step t mu t' mu' -> step (Ref t) mu (Ref t') mu'
-  | S_RefV     : forall v mu, value v -> step (Ref v) mu (Loc (length mu)) ((length mu, v) :: mu)
-  | S_Deref    : forall t mu t' mu', step t mu t' mu' -> step (Deref t) mu (Deref t') mu'
+  | S_IsZero : forall t mu t' mu', step t mu t' mu' -> step (IsZero t) mu (IsZero t') mu'
+  | S_IfTrue : forall t1 t2 mu, step (If (BOOL true) t1 t2) mu t1 mu
+  | S_IfFalse : forall t1 t2 mu, step (If (BOOL false) t1 t2) mu t2 mu
+  | S_If : forall t1 mu t1' mu' t2 t3, step t1 mu t1' mu' -> step (If t1 t2 t3) mu (If t1' t2 t3) mu'
+  | S_App1 : forall t1 mu t1' mu' t2, step t1 mu t1' mu' -> step (App t1 t2) mu (App t1' t2) mu'
+  | S_App2 : forall v1 t2 mu t2' mu', value v1 -> step t2 mu t2' mu' -> step (App v1 t2) mu (App v1 t2') mu'
+  | S_AppAbs : forall T t1 v2 mu, value v2 -> step (App (Lam T t1) v2) mu (subst 0 v2 t1) mu
+  | S_Fix : forall t mu, step (Fix t) mu (subst 0 (Fix t) t) mu
+  | S_Ref : forall t mu t' mu', step t mu t' mu' -> step (Ref t) mu (Ref t') mu'
+  | S_RefV : forall v mu, value v -> step (Ref v) mu (Loc (length mu)) ((length mu, v) :: mu)
+  | S_Deref : forall t mu t' mu', step t mu t' mu' -> step (Deref t) mu (Deref t') mu'
   | S_DerefLoc : forall l mu v, heap_lookup l mu = Some v -> step (Deref (Loc l)) mu v mu
-  | S_Assign1  : forall t1 mu t1' mu' t2, step t1 mu t1' mu' -> step (Assign t1 t2) mu (Assign t1' t2) mu'
-  | S_Assign2  : forall l t2 mu t2' mu', step t2 mu t2' mu' -> step (Assign (Loc l) t2) mu (Assign (Loc l) t2') mu'
-  | S_AssignV  : forall l v mu, value v -> step (Assign (Loc l) v) mu (Num 0) (heap_update l v mu).
+  | S_Assign1 : forall t1 mu t1' mu' t2, step t1 mu t1' mu' -> step (Assign t1 t2) mu (Assign t1' t2) mu'
+  | S_Assign2 : forall l t2 mu t2' mu', step t2 mu t2' mu' -> step (Assign (Loc l) t2) mu (Assign (Loc l) t2') mu'
+  | S_AssignV : forall l v mu, value v -> step (Assign (Loc l) v) mu (Num 0) (heap_update l v mu).
 
 Definition extends (S' S : store_ty) : Prop := exists S2, S' = S ++ S2.
 
+(** * Lemmas for the preservation proof *)
 
-Lemma substitution_preserves_typing : forall G S t T U s, has_type (G ++ U :: []) S t T -> has_type G S s U -> has_type G S (subst (length G) s t) T.
+Lemma nth_error_app_prefix : forall A (G1 G2 : list A) (x : nat) (T' : A),
+  x < length G1 -> nth_error (G1 ++ T' :: G2) x = nth_error G1 x.
 Proof.
-Admitted.
+  induction G1; simpl; intros. lia.
+  destruct x; simpl; auto. apply IHG1. lia.
+Qed.
+
+Lemma nth_error_app_suffix : forall A (G1 G2 : list A) (x : nat) (T' : A) T,
+  length G1 <= x ->
+  nth_error (G1 ++ G2) x = Some T ->
+  nth_error (G1 ++ T' :: G2) (x + 1) = Some T.
+Proof.
+  induction G1; simpl; intros. apply H0.
+  destruct x. lia. simpl. apply IHG1. lia. apply H0.
+Qed.
+
+Lemma shift_at_preserves_typing : forall G1 G2 S t T T',
+  has_type (G1 ++ G2) S t T ->
+  has_type (G1 ++ T' :: G2) S (shift_at (length G1) t) T.
+Proof.
+  intros G1 G2 S t T T' Hty.
+  remember (G1 ++ G2) as Gamma.
+  generalize dependent G2. generalize dependent G1.
+  induction Hty; simpl; intros G1' G2' Heq; subst Gamma.
+  - (* T_Var *)
+    rename H into Hnth.
+    destruct (Nat.ltb_spec x (length G1')).
+    + apply T_Var. rewrite nth_error_app_prefix by auto. exact Hnth.
+    + apply T_Var. eapply nth_error_app_suffix; eauto. lia.
+  - apply T_Num.
+  - apply T_Bool.
+  - apply T_Succ; eauto.
+  - apply T_Pred; eauto.
+  - apply T_IsZero; eauto.
+  - apply T_If; eauto.
+  - (* T_Lam *)
+    apply T_Lam.
+    replace (T1 :: G1' ++ T' :: G2') with ((T1 :: G1') ++ T' :: G2') by reflexivity.
+    apply (IHHty (T1 :: G1') G2'). simpl. rewrite Heq. reflexivity.
+  - apply T_App with T1; eauto.
+  - (* T_Fix *)
+    apply T_Fix.
+    replace (T0 :: G1' ++ T' :: G2') with ((T0 :: G1') ++ T' :: G2') by reflexivity.
+    apply (IHHty (T0 :: G1') G2'). simpl. rewrite Heq. reflexivity.
+  - apply T_Ref; eauto.
+  - apply T_Deref; eauto.
+  - apply T_Assign with T; eauto.
+  - apply T_Loc. exact H.
+Qed.
+
+Lemma shift_preserves_typing : forall T' G S t T,
+  has_type G S t T -> has_type (T' :: G) S (shift t) T.
+Proof.
+  intros. apply (shift_at_preserves_typing [] G S t T T'); simpl; auto.
+Qed.
+
+Lemma substitution_preserves_typing : forall G S t T U s,
+  has_type (G ++ [U]) S t T ->
+  has_type G S s U ->
+  has_type G S (subst (length G) s t) T.
+Proof.
+  intros G S t T U s Hty Hs.
+  remember (G ++ [U]) as Gamma.
+  generalize dependent s.
+  generalize dependent G.
+  induction Hty; intros G' Heq s' Hs'; subst Gamma; simpl.
+  - (* T_Var *)
+    rename H into Hnth.
+    destruct (Nat.ltb_spec x (length G')).
+    + (* x < length G' *)
+      rewrite nth_error_app_prefix with (T' := U) (G1 := G') (G2 := []) in Hnth by auto.
+      apply T_Var. exact Hnth.
+    + (* x >= length G', so x = length G' since G++[U] has length G+1 *)
+      apply T_Var.
+      replace (length G') with x by lia.
+      apply nth_error_app_suffix with (G1 := G') (G2 := []) (T' := U); auto.
+      lia. exact Hnth.
+  - apply T_Num.
+  - apply T_Bool.
+  - apply T_Succ; apply IHHty with (G := G'); auto.
+  - apply T_Pred; apply IHHty with (G := G'); auto.
+  - apply T_IsZero; apply IHHty with (G := G'); auto.
+  - apply T_If; [apply IHHty1 with (G := G') | apply IHHty2 with (G := G') | apply IHHty3 with (G := G')]; auto.
+  - (* T_Lam *)
+    apply T_Lam.
+    replace (T1 :: G' ++ [U]) with ((T1 :: G') ++ [U]) by reflexivity.
+    apply (IHHty (T1 :: G')); auto.
+    simpl. reflexivity.
+    apply shift_preserves_typing. auto.
+  - apply T_App with T1; [apply IHHty1 with (G := G') | apply IHHty2 with (G := G')]; auto.
+  - (* T_Fix *)
+    apply T_Fix.
+    replace (T0 :: G' ++ [U]) with ((T0 :: G') ++ [U]) by reflexivity.
+    apply (IHHty (T0 :: G')); auto.
+    simpl. reflexivity.
+    apply shift_preserves_typing. auto.
+  - apply T_Ref; apply IHHty with (G := G'); auto.
+  - apply T_Deref; apply IHHty with (G := G'); auto.
+  - apply T_Assign with T; [apply IHHty1 with (G := G') | apply IHHty2 with (G := G')]; auto.
+  - apply T_Loc. exact H.
+Qed.
+
+(** * Type Preservation *)
 
 Theorem preservation :
   forall t mu t' mu' T S,
@@ -132,13 +247,21 @@ Proof.
   - (* S_If *) inversion Hty; subst. destruct (IHHstep TyBool S H3 Hok) as [S' [? [? ?]]]. exists S'; eauto.
   - (* S_App1 *) inversion Hty; subst. destruct (IHHstep (TyArrow T1 T0) S H3 Hok) as [S' [? [? ?]]]. exists S'; eauto.
   - (* S_App2 *) inversion Hty; subst. destruct (IHHstep T1 S H5 Hok) as [S' [? [? ?]]]. exists S'; eauto.
-  - (* S_AppAbs *) admit.
-  - (* S_Fix *) admit.
+  - (* S_AppAbs *)
+    inversion Hty; subst. inversion H0; subst.
+    exists S. unfold extends. exists []. split; [apply app_nil_r|].
+    split; [exact Hok|].
+    eapply substitution_preserves_typing with (G := []); simpl; eauto.
+  - (* S_Fix *)
+    inversion Hty; subst.
+    exists S. unfold extends. exists []. split; [apply app_nil_r|].
+    split; [exact Hok|].
+    eapply substitution_preserves_typing with (G := []); simpl; eauto.
   - (* S_Ref *) inversion Hty; subst. destruct (IHHstep T0 S H2 Hok) as [S' [? [? ?]]]. exists S'; eauto.
-  - (* S_RefV *) inversion Hty; subst. inversion H0; subst. exists (S ++ [T0]). unfold extends. repeat split; eauto. { exists [T0]. reflexivity. } { induction Hok. constructor. eapply heap_cons with (T:=T). apply IHHok. apply H1. apply nth_error_app_l. apply H3. } { apply T_Loc. apply nth_error_last. }
+  - (* S_RefV *) inversion Hty; subst. inversion H0; subst. exists (S ++ [T0]). unfold extends. repeat split; eauto. { exists [T0]. reflexivity. } { induction Hok. constructor. eapply heap_cons with (T := T). apply IHHok. apply H1. apply nth_error_app_l. apply H3. } { apply T_Loc. apply nth_error_last. }
   - (* S_Deref *) inversion Hty; subst. destruct (IHHstep (TyRef T0) S H2 Hok) as [S' [? [? ?]]]. exists S'; eauto.
   - (* S_DerefLoc *) inversion Hty; subst. inversion H0; subst. induction Hok; simpl in *. discriminate. destruct (Nat.eqb l l0) eqn:Heq. injection H; intros; subst. exists S; eauto. apply IHHok; auto.
   - (* S_Assign1 *) inversion Hty; subst. destruct (IHHstep (TyRef T1) S H2 Hok) as [S' [? [? ?]]]. exists S'; eauto.
   - (* S_Assign2 *) inversion Hty; subst. destruct (IHHstep T1 S H4 Hok) as [S' [? [? ?]]]. exists S'; eauto.
-  - (* S_AssignV *) inversion Hty; subst. inversion H0; subst. exists S. repeat split; eauto. { induction Hok. constructor. destruct (Nat.eqb l0 l) eqn:Heq. subst. rewrite Nat.eqb_refl. apply heap_cons with (T:=T0); auto. rewrite H3 in H1. injection H1; intros; subst; auto. rewrite Nat.eqb_sym. rewrite Heq. apply heap_cons with (T:=T); auto. } { apply T_Num. }
-Admitted.
+  - (* S_AssignV *) inversion Hty; subst. inversion H0; subst. exists S. repeat split; eauto. { induction Hok. constructor. destruct (Nat.eqb l0 l) eqn:Heq. subst. rewrite Nat.eqb_refl. apply heap_cons with (T := T0); auto. rewrite H3 in H1. injection H1; intros; subst; auto. rewrite Nat.eqb_sym. rewrite Heq. apply heap_cons with (T := T); auto. } { apply T_Num. }
+Qed.
